iris: PipeLinks -- the pipeline's link bundle IS its record equation (app-both M3c, third cut)
pipe_links g := the pure equation riscv_cons_res = pecl g (pipe_links_eq
reads it back).  The leaves consumers spend by name (pipe_link_taint, _rd,
_rd_taint, _file) are read off it through the link lemmas; M2's write
interface (PipeLinksLine.pipe_links_gl) calls pipe_write_link(_blk/_pro) at
the equation.  The seven-field bundle, its w/blk/pro fields and the
projections that only fed pipe_links_gl are gone.  The pipe's links stay
pipe-own (its claim has the open-round arm, so GenLinks does not apply).

Co-Authored-By: Claude Opus 5.5 (1M context) <noreply@anthropic.com>

iris/PipeLinks.v
@@ -295,60 +295,48 @@ Section pipe_links.
   Qed.
 
   (* ==================================================================== *)
-  (*  THE BUNDLE.  [EchoLinks.echo_links]'s shape at this claim: the six   *)
-  (*  links as CLOSED [box] wands with their Coq-level premises turned     *)
-  (*  into [pure] wands, so the whole thing is ONE [iProp] a program holds  *)
-  (*  and spends per byte, and the record equations stay where             *)
-  (*  [App.al_echo] hands them over.  SIX and not seven: there is no       *)
-  (*  boot-state-filing first byte.                                       *)
+  (*  THE ECHO SHIFT ITSELF -- [App.al_echo], a CLOSED entailment.         *)
   (* ==================================================================== *)
-  Definition pipe_link_w : iProp Σ :=
-    (□ ∀ (k : nat) (v : era_pins) (P : nat) (b : bv 8)
-         (ps0 cs0 : list nat) (I0 : list (bv 8)) (Φ : iProp Σ),
-        ⌜(nlines I0 <= length cs0)%nat⌝ -∗
-        ⌜pro_pin_p ps0 cs0 I0⌝ -∗
-        ⌜proc_stream_p ps0 cs0 I0 !! P = Some b⌝ -∗
-        era_pin γ k v -∗ turn v P -∗
-        ps_lb v ps0 -∗ cs_lb v cs0 -∗ inp_lb v I0 -∗
-        (((turn v (S P) ∗ ps_lb v ps0 ∗ cs_lb v cs0 ∗ inp_lb v I0)
-          ∨ T) -∗ Φ) -∗
-        out_link Uart0 k b Φ)%I.
+  Lemma pipe_happ_echo :
+    ⊢ ∀ (GEN : GenId) (XI : CurCtx),
+        @SpecConsoleintr.cons_echo_shift Σ HRg GEN XI.
+  Proof using Hcons Htag.
+    iIntros (GEN XI).
+    rewrite /SpecConsoleintr.cons_echo_shift Htag.
+    iIntros "!>" (h c cs Φ) "%Hends %Hk %Hcs #Htg #Hlbh HΦ".
+    iDestruct "Htg" as "[%Hsh [%Hdisc | #HT]]"; last first.
+    { iApply (pipe_cons_link_of_taint with "HT [HΦ]").
+      by iApply pipe_cons_run. }
+    iIntros (o H) "#Hlb Hres %Hok %Hev".
+    rewrite pchist_at0.
+    iDestruct (pecl_open g (S gen_id) (default [] o) H h c cs Hok Hev
+                 (disc_seg_p_open_seg h Hsh Hdisc) Hk Hdisc Hsh
+                 with "Hres") as "Hres".
+    iModIntro. iExists (Some h). cbn [obs_hist_lb_o from_option id].
+    rewrite pchist_at0. iFrame "Hlbh Hres".
+    by iApply pipe_cons_run.
+  Qed.
 
-  Definition pipe_link_blk : iProp Σ :=
-    (□ ∀ (k : nat) (v : era_pins) (P a : nat) (b : bv 8)
-         (ps0 cs0 : list nat) (I0 : list (bv 8)) (Φ : iProp Σ),
-        ⌜I0 <> []⌝ -∗
-        ⌜rest_of I0 = []⌝ -∗
-        ⌜(nlines I0 <= S (length cs0))%nat⌝ -∗
-        ⌜pro_pin_p ps0 cs0 I0⌝ -∗
-        ⌜P = length (proc_before_p ps0 cs0 I0)⌝ -∗
-        ⌜palt_ok (pline_of (bodies_of I0 !!! (nlines I0 - 1)%nat))
-                 (palt_of a)⌝ -∗
-        ⌜palt_isforkS (palt_of a) = false⌝ -∗
-        ⌜pcont (pline_of (bodies_of I0 !!! (nlines I0 - 1)%nat)) (palt_of a)
-           !! 0%nat = Some b⌝ -∗
-        era_pin γ k v -∗ turn v P -∗
-        ps_lb v ps0 -∗ cs_lb v cs0 -∗ inp_lb v I0 -∗
-        (((turn v (S P) ∗ ps_lb v ps0 ∗ cs_lb v (cs0 ++ [a]) ∗ inp_lb v I0)
-          ∨ T) -∗ Φ) -∗
-        out_link Uart0 k b Φ)%I.
+End pipe_links.
 
-  Definition pipe_link_pro : iProp Σ :=
-    (□ ∀ (k : nat) (v : era_pins) (P a : nat) (b : bv 8)
-         (ps0 cs0 : list nat) (I0 : list (bv 8)) (Φ : iProp Σ),
-        ⌜rest_of I0 = []⌝ -∗
-        ⌜I0 = [] \/ palt_panic (palt_at cs0 (nlines I0 - 1)%nat) = true⌝ -∗
-        ⌜(nlines I0 <= length cs0)%nat⌝ -∗
-        ⌜pro_pin_p ps0 cs0 I0⌝ -∗
-        ⌜~ pro_done (pro_from (pro_idx_p cs0 (nlines I0)) ps0)⌝ -∗
-        ⌜P = length (proc_stream_p ps0 cs0 I0)⌝ -∗
-        ⌜(a < length pro_alts)%nat⌝ -∗
-        ⌜pro_alts !!! a !! 0%nat = Some b⌝ -∗
-        era_pin γ k v -∗ turn v P -∗
-        ps_lb v ps0 -∗ cs_lb v cs0 -∗ inp_lb v I0 -∗
-        (((turn v (S P) ∗ ps_lb v (ps0 ++ [a]) ∗ cs_lb v cs0 ∗ inp_lb v I0)
-          ∨ T) -∗ Φ) -∗
-        out_link Uart0 k b Φ)%I.
+(* ====================================================================== *)
+(*  THE BUNDLE.  The pipeline's links are what the record equation gives: *)
+(*  every console link of the era is one of the lemmas above once the     *)
+(*  console record's claim is [pecl g].  So the bundle a program holds    *)
+(*  and spends is the EQUATION ITSELF, as a pure persistent fact, and the *)
+(*  links are read off it where they are spent (the leaves below, and     *)
+(*  M2's write interface in [PipeLinksLine.pipe_links_gl]).  The record   *)
+(*  equations stay where [App.al_echo] hands them over.                   *)
+(* ====================================================================== *)
+Section pipe_links_bundle.
+  Context {Σ : gFunctors}.
+  Context `{!echoOutG Σ}.
+  Context `{!pipeOutG Σ}.
+  Context (g : pipe_gn).
+  Local Notation γ := (pgn_cl g).
+  Context `{HRg : !riscvGS Σ}.
+
+  Notation T := (echo_taint γ).
 
   Definition pipe_link_taint : iProp Σ :=
     (□ ∀ (k : nat) (b : bv 8) (Φ : iProp Σ),
@@ -358,7 +346,7 @@ Section pipe_links.
     (□ ∀ (k : nat) (v : era_pins) (n : nat)
          (ws : list (list mobs * bv 8)) (Φ : iProp Σ),
         era_pin γ k v -∗ dl_cnt v (1/2) n -∗
-        (pread_ret k v n ws -∗ Φ) -∗
+        (pread_ret g k v n ws -∗ Φ) -∗
         cons_link Uart0 k (ConsLog.EvRead ws) Φ)%I.
 
   Definition pipe_link_rd_taint : iProp Σ :=
@@ -389,15 +377,8 @@ Section pipe_links.
         out_link Uart0 k b Phi)%I.
 
   Definition pipe_links : iProp Σ :=
-    (pipe_link_w ∗ pipe_link_blk ∗ pipe_link_pro ∗ pipe_link_taint
-     ∗ pipe_link_rd ∗ pipe_link_rd_taint ∗ pipe_link_file)%I.
+    ⌜@riscv_cons_res Σ (@riscv_fixedGS Σ HRg) = pecl g⌝%I.
 
-  Global Instance pipe_link_w_persistent : Persistent pipe_link_w | 0.
-  Proof using . rewrite /pipe_link_w. apply _. Qed.
-  Global Instance pipe_link_blk_persistent : Persistent pipe_link_blk | 0.
-  Proof using . rewrite /pipe_link_blk. apply _. Qed.
-  Global Instance pipe_link_pro_persistent : Persistent pipe_link_pro | 0.
-  Proof using . rewrite /pipe_link_pro. apply _. Qed.
   Global Instance pipe_link_taint_persistent : Persistent pipe_link_taint | 0.
   Proof using . rewrite /pipe_link_taint. apply _. Qed.
   Global Instance pipe_link_rd_persistent : Persistent pipe_link_rd | 0.
@@ -410,81 +391,53 @@ Section pipe_links.
   Global Instance pipe_links_persistent : Persistent pipe_links | 0.
   Proof using . rewrite /pipe_links. apply _. Qed.
 
-  (* ---- the seven projections, which is all a consumer ever uses ---- *)
-  Lemma pipe_links_w : pipe_links -∗ pipe_link_w.
-  Proof using . by iIntros "($ & _ & _ & _ & _ & _ & _)". Qed.
-  Lemma pipe_links_blk : pipe_links -∗ pipe_link_blk.
-  Proof using . by iIntros "(_ & $ & _ & _ & _ & _ & _)". Qed.
-  Lemma pipe_links_pro : pipe_links -∗ pipe_link_pro.
-  Proof using . by iIntros "(_ & _ & $ & _ & _ & _ & _)". Qed.
+  (* the equation, read back out *)
+  Lemma pipe_links_eq :
+    pipe_links -∗ ⌜@riscv_cons_res Σ (@riscv_fixedGS Σ HRg) = pecl g⌝.
+  Proof using . rewrite /pipe_links. by iIntros "%Hc". Qed.
+
+  (* ---- the leaves a consumer spends ---- *)
   Lemma pipe_links_taint : pipe_links -∗ pipe_link_taint.
-  Proof using . by iIntros "(_ & _ & _ & $ & _ & _ & _)". Qed.
+  Proof using .
+    iIntros "Hlk". iDestruct (pipe_links_eq with "Hlk") as %Hc.
+    rewrite /pipe_link_taint. iIntros "!>" (k b Φ) "HT HΦ".
+    iApply (pipe_write_link_taint g Hc with "HT HΦ").
+  Qed.
+
   Lemma pipe_links_rd : pipe_links -∗ pipe_link_rd.
-  Proof using . by iIntros "(_ & _ & _ & _ & $ & _ & _)". Qed.
+  Proof using .
+    iIntros "Hlk". iDestruct (pipe_links_eq with "Hlk") as %Hc.
+    rewrite /pipe_link_rd. iIntros "!>" (k v n ws Φ) "Hpin Hdl HΦ".
+    iApply (pipe_read_link g Hc with "Hpin Hdl HΦ").
+  Qed.
+
   Lemma pipe_links_rd_taint : pipe_links -∗ pipe_link_rd_taint.
-  Proof using . by iIntros "(_ & _ & _ & _ & _ & $ & _)". Qed.
+  Proof using .
+    iIntros "Hlk". iDestruct (pipe_links_eq with "Hlk") as %Hc.
+    rewrite /pipe_link_rd_taint. iIntros "!>" (k ws Φ) "#HT HΦ".
+    iApply (pipe_cons_link_of_taint g Hc with "HT [HΦ]").
+    by iApply "HΦ".
+  Qed.
+
   Lemma pipe_links_file : pipe_links -∗ pipe_link_file.
-  Proof using . by iIntros "(_ & _ & _ & _ & _ & _ & $)". Qed.
-
-  Lemma pipe_links_holds : ⊢ pipe_links.
-  Proof using Hcons.
-    rewrite /pipe_links /pipe_link_w /pipe_link_blk /pipe_link_pro
-            /pipe_link_taint /pipe_link_rd /pipe_link_rd_taint
-            /pipe_link_file.
-    iSplit; [| iSplit; [| iSplit; [| iSplit; [| iSplit; [| iSplit]]]]].
-    - iIntros "!>" (k v P b ps0 cs0 I0 Φ) "%Hbnd %Hpin0 %Hb".
-      iIntros "Hpin Ht Hps Hcs HE HΦ".
-      iApply (pipe_write_link with "Hpin Ht Hps Hcs HE HΦ"); try assumption.
-    - iIntros "!>" (k v P a b ps0 cs0 I0 Φ).
-      iIntros "%Hne %Hrest %Hbnd %Hpin0 %HPeq %Halt %Hfk %Hhead".
-      iIntros "Hpin Ht Hps Hcs HE HΦ".
-      iApply (pipe_write_link_blk with "Hpin Ht Hps Hcs HE HΦ");
-        try assumption.
-    - iIntros "!>" (k v P a b ps0 cs0 I0 Φ).
-      iIntros "%Hrest %Hopen %Hbnd %Hpin0 %Hnd %HPeq %Halt %Hhead".
-      iIntros "Hpin Ht Hps Hcs HE HΦ".
-      iApply (pipe_write_link_pro with "Hpin Ht Hps Hcs HE HΦ");
-        try assumption.
-    - iIntros "!>" (k b Φ) "HT HΦ".
-      iApply (pipe_write_link_taint with "HT HΦ").
-    - iIntros "!>" (k v n ws Φ) "Hpin Hdl HΦ".
-      iApply (pipe_read_link with "Hpin Hdl HΦ").
-    - iIntros "!>" (k ws Φ) "#HT HΦ".
-      iApply (pipe_cons_link_of_taint with "HT [HΦ]").
-      by iApply "HΦ".
-    - iIntros "!>" (k v w gb P r a b pre0 ps0 cs0 I0 Phi).
-      iIntros "%Hne %Hrest %Hreq %Hcseq %Hpin0 %HPeq %Halt %Hpan %Hfk %Hcont %Hbv".
-      iIntros "Hpin Hpera Ht Hcw Hrlb Hps Hcs HE HPhi".
-      iApply (pipe_file_link with "Hpin Hpera Ht Hcw Hrlb Hps Hcs HE HPhi");
-        try assumption.
+  Proof using .
+    iIntros "Hlk". iDestruct (pipe_links_eq with "Hlk") as %Hc.
+    rewrite /pipe_link_file.
+    iIntros "!>" (k v w gb P r a b pre0 ps0 cs0 I0 Phi).
+    iIntros "%Hne %Hrest %Hreq %Hcseq %Hpin0 %HPeq %Halt %Hpan %Hfk %Hcont %Hbv".
+    iIntros "Hpin Hpera Ht Hcw Hrlb Hps Hcs HE HPhi".
+    iApply (pipe_file_link g Hc with "Hpin Hpera Ht Hcw Hrlb Hps Hcs HE HPhi");
+      try assumption.
   Qed.
 
-  (* ==================================================================== *)
-  (*  THE ECHO SHIFT ITSELF -- [App.al_echo], a CLOSED entailment.         *)
-  (* ==================================================================== *)
-  Lemma pipe_happ_echo :
-    ⊢ ∀ (GEN : GenId) (XI : CurCtx),
-        @SpecConsoleintr.cons_echo_shift Σ HRg GEN XI.
-  Proof using Hcons Htag.
-    iIntros (GEN XI).
-    rewrite /SpecConsoleintr.cons_echo_shift Htag.
-    iIntros "!>" (h c cs Φ) "%Hends %Hk %Hcs #Htg #Hlbh HΦ".
-    iDestruct "Htg" as "[%Hsh [%Hdisc | #HT]]"; last first.
-    { iApply (pipe_cons_link_of_taint with "HT [HΦ]").
-      by iApply pipe_cons_run. }
-    iIntros (o H) "#Hlb Hres %Hok %Hev".
-    rewrite pchist_at0.
-    iDestruct (pecl_open g (S gen_id) (default [] o) H h c cs Hok Hev
-                 (disc_seg_p_open_seg h Hsh Hdisc) Hk Hdisc Hsh
-                 with "Hres") as "Hres".
-    iModIntro. iExists (Some h). cbn [obs_hist_lb_o from_option id].
-    rewrite pchist_at0. iFrame "Hlbh Hres".
-    by iApply pipe_cons_run.
-  Qed.
+  Lemma pipe_links_holds
+      (Hcons : @riscv_cons_res Σ (@riscv_fixedGS Σ HRg) = pecl g) :
+    ⊢ pipe_links.
+  Proof using . by iPureIntro. Qed.
+End pipe_links_bundle.
 
-End pipe_links.
-
-(* PIPE-2W-3: THE BUNDLE IS OPAQUE TO THE INSTANCE SEARCH.  [pipe_links] is
+(* PIPE-2W-3: THE BUNDLE IS OPAQUE TO THE INSTANCE SEARCH (kept now that
+   the bundle is the record equation: consumers name the instance).  It was
    a six-fold [∗] of wand bundles; left transparent, the [Persistent] search
    UNFOLDS it instead of taking [pipe_links_persistent], and then descends
    into the wands -- the tree's documented "a bundle of wands hangs the
@@ -496,7 +449,7 @@ End pipe_links.
    constants are opaque to the search, so a [Persistent (pipe_links _)] goal
    is settled by its own instance and nothing else is tried. *)
 #[global] Typeclasses Opaque pipe_links.
-(* ONLY THE BUNDLE.  The six links themselves stay transparent: each is
+(* ONLY THE BUNDLE.  The leaves themselves stay transparent: each is
    [□ ∀ ...], so its own [Persistent] is one step, and [iSpecialize] /
    [iApply ("Ht" $! k b Φ)] must be able to see the [∀] through the name
    (made them opaque once -- PipeLinksLine.v:1406 answered with
